Phi_Algebras/Phi_Fiction.thy
@@ -1,0 +1,282 @@
+theory Phi_Fiction
+  imports Algebras
+begin
+
+section \<open>Interpretation of Fictional Separation\<close>
+
+subsection \<open>Algebric Structure\<close>
+
+text \<open>
+  Referring to Fictional Separation Logic~\cite{FSL}, the interpretation of fictional separation
+  maps a fictional resource to a set of concrete resource.
+  The interpretation can be any map to set that preserves \<open>1\<close>, the unit of the separation algebra.\<close>
+
+definition Interpretation :: "('a::one \<Rightarrow> 'b::one set) \<Rightarrow> bool"
+  where "Interpretation \<I> \<longleftrightarrow> \<I> 1 = 1"
+
+typedef (overloaded) ('a::one,'b::one) interp
+    = \<open>Collect (Interpretation :: ('a \<Rightarrow> 'b set) \<Rightarrow> bool)\<close>
+  morphisms \<I> Interp
+  by (rule exI[where x = \<open>\<lambda>_. 1\<close>]) (simp add:sep_mult_commute Interpretation_def)
+
+text \<open>Type \<open>('a,'b) interp\<close> encapsulating the 1-preserving condition, represents an interpretation.
+\<^const>\<open>\<I>\<close> activates the interpretation; \<^const>\<open>Interp\<close> constructs an interpretation by checking
+the 1-preserving condition.
+\[@{thm Interp_inverse[simplified]}\]\<close>
+
+lemmas Interp_inverse[simp] = Interp_inverse[simplified]
+
+lemma Interp_one[simp]: "\<I> I 1 = 1"
+  using Interpretation_def \<I> by blast
+
+definition \<I>\<^sub>r\<^sub>e\<^sub>l :: \<open>('a::one,'b::one) interp \<Rightarrow> ('a \<times> 'b) set\<close> 
+  where \<open>\<I>\<^sub>r\<^sub>e\<^sub>l I = {(x,y). y \<in> \<I> I x}\<close>
+
+
+
+definition Fictional_Forward_Simulation :: \<open>'c rel \<Rightarrow> 'a rel \<Rightarrow> ('a::sep_magma_1,'c::sep_magma_1) interp \<Rightarrow> 'a set \<Rightarrow> bool\<close>
+      ("_/ \<r>\<e>\<f>\<i>\<n>\<e>\<s> _/ \<w>.\<r>.\<t> _/ \<i>\<n> _" [11,11,11] 10)
+  where \<open>(F \<r>\<e>\<f>\<i>\<n>\<e>\<s> G \<w>.\<r>.\<t> T \<i>\<n> D) \<longleftrightarrow> (\<forall>x r R. F `` (R * \<I> T (r * x) \<s>\<u>\<b>\<j> r ## x \<and> x \<in> D) \<subseteq> { y'. \<exists>y. y' \<in> R * \<I> T (r * y) \<and> r ## y \<and> (x,y) \<in> G})\<close>
+
+definition \<open>refinement_projection I D = \<Union> (\<I> I ` (UNIV * D))\<close>
+
+lemma empty_refines_any[simp]:
+  \<open>{} \<r>\<e>\<f>\<i>\<n>\<e>\<s> Any \<w>.\<r>.\<t> I \<i>\<n> D\<close>
+  unfolding Fictional_Forward_Simulation_def
+  by simp
+
+lemma refinement_sub_domain:
+  \<open> D' \<subseteq> D
+\<Longrightarrow> A \<r>\<e>\<f>\<i>\<n>\<e>\<s> B \<w>.\<r>.\<t> I \<i>\<n> D
+\<Longrightarrow> A \<r>\<e>\<f>\<i>\<n>\<e>\<s> B \<w>.\<r>.\<t> I \<i>\<n> D'\<close>
+  unfolding Fictional_Forward_Simulation_def
+  by (clarsimp simp add: Subjection_expn subset_iff Image_def Bex_def Id_on_iff, blast)
+
+lemma refinement_sub_fun:
+  \<open> A' \<subseteq> A
+\<Longrightarrow> A  \<r>\<e>\<f>\<i>\<n>\<e>\<s> B \<w>.\<r>.\<t> I \<i>\<n> D
+\<Longrightarrow> A' \<r>\<e>\<f>\<i>\<n>\<e>\<s> B \<w>.\<r>.\<t> I \<i>\<n> D\<close>
+  unfolding Fictional_Forward_Simulation_def
+  by (clarsimp simp add: Subjection_expn subset_iff Image_def Bex_def Id_on_iff; blast)
+
+lemma refinement_sub_fun_right:
+  \<open> B \<subseteq> B'
+\<Longrightarrow> A  \<r>\<e>\<f>\<i>\<n>\<e>\<s> B \<w>.\<r>.\<t> I \<i>\<n> D
+\<Longrightarrow> A \<r>\<e>\<f>\<i>\<n>\<e>\<s> B' \<w>.\<r>.\<t> I \<i>\<n> D\<close>
+  unfolding Fictional_Forward_Simulation_def
+  by (clarsimp simp add: Subjection_expn subset_iff Image_def Bex_def Id_on_iff; blast)
+
+lemma refinement_frame:
+  \<open> A \<r>\<e>\<f>\<i>\<n>\<e>\<s> B \<w>.\<r>.\<t> I \<i>\<n> D
+\<Longrightarrow> A \<r>\<e>\<f>\<i>\<n>\<e>\<s> Id_on R * B \<w>.\<r>.\<t> I \<i>\<n> R * D\<close>
+  for B :: \<open>'b::sep_monoid rel\<close>
+  unfolding Fictional_Forward_Simulation_def
+  apply (clarsimp simp add: subset_iff Subjection_expn set_mult_expn Image_def Bex_def Id_on_iff)
+  by (smt (z3) sep_disj_multD1 sep_disj_multD2 sep_disj_multI1 sep_disj_multI2 sep_mult_assoc')
+
+
+
+
+
+subsection \<open>Instances\<close>
+
+subsubsection \<open>Identity\<close>
+
+definition [simp]: "\<F>_it' x = {x}"
+
+definition "\<F>_it = Interp \<F>_it'"
+
+lemma \<F>_it_\<I>[simp]: "\<I> \<F>_it = \<F>_it'"
+  unfolding \<F>_it_def
+  by (rule Interp_inverse) (simp add: Interpretation_def one_set_def)
+
+
+
+subsubsection \<open>Composition\<close>
+
+definition interp_comp :: \<open>('b::one,'c::one) interp \<Rightarrow> ('a::one,'b) interp \<Rightarrow> ('a,'c) interp\<close> (infixr "\<circ>\<^sub>\<I>" 55)
+  where \<open>(I1 \<circ>\<^sub>\<I> I2) = Interp (\<lambda>x. \<Union>(\<I> I1 ` \<I> I2 x))\<close>
+
+notation interp_comp  (infixl "o\<^sub>\<I>" 55)
+
+lemma interp_comp_\<I>[simp]:
+  \<open>\<I> (I1 \<circ>\<^sub>\<I> I2) = (\<lambda>x. \<Union>(\<I> I1 ` \<I> I2 x))\<close>
+  unfolding interp_comp_def
+  by (rule Interp_inverse)  (simp add: Interpretation_def one_set_def)
+
+lemma interp_comp_assoc:
+  \<open>(I1 \<circ>\<^sub>\<I> I2) \<circ>\<^sub>\<I> I3 = I1 \<circ>\<^sub>\<I> (I2 \<circ>\<^sub>\<I> I3)\<close>
+  by (subst \<I>_inject[symmetric]; simp)
+
+lemma \<F>_it_comp[simp]:
+  \<open>\<F>_it o\<^sub>\<I> I = I\<close> \<open>I o\<^sub>\<I> \<F>_it = I\<close>
+  by (subst \<I>_inject[symmetric], simp)+
+
+lemma sep_refinement_stepwise:
+  \<open> S1 \<r>\<e>\<f>\<i>\<n>\<e>\<s> S2 \<w>.\<r>.\<t> I1 \<i>\<n> D
+\<Longrightarrow> S2 \<r>\<e>\<f>\<i>\<n>\<e>\<s> S3 \<w>.\<r>.\<t> I2 \<i>\<n> D'
+\<Longrightarrow> refinement_projection I2 D' \<subseteq> D
+\<Longrightarrow> S1 \<r>\<e>\<f>\<i>\<n>\<e>\<s> S3 \<w>.\<r>.\<t> (I1 o\<^sub>\<I> I2) \<i>\<n> D'\<close>
+  unfolding Fictional_Forward_Simulation_def interp_comp_\<I> refinement_projection_def
+  apply (auto simp add: subset_iff Image_def Bex_def Subjection_expn set_mult_expn split_option_all)
+  subgoal premises prems for x r R t u v xb
+  proof -
+    thm prems
+    thm prems(1)[THEN spec[where x=xb],THEN spec[where x=1],THEN spec[where x=\<open>R\<close>],THEN spec[where x=\<open>t\<close>]]
+    have \<open>(\<exists>x. (\<exists>u v. x = u * v \<and> u \<in> R \<and> v \<in> \<I> I1 (1 * xb) \<and> u ## v) \<and> 1 ## xb \<and> xb \<in> D \<and> (x, t) \<in> S1)\<close>
+      apply (simp add: prems)
+      using prems(10) prems(3) prems(4) prems(5) prems(6) prems(7) prems(8) prems(9) by blast
+    note prems(1)[THEN spec[where x=xb],THEN spec[where x=1],THEN spec[where x=\<open>R\<close>],THEN spec[where x=\<open>t\<close>],
+          THEN mp, OF this]
+    then show ?thesis
+      apply clarsimp
+      subgoal premises prems2 for y u'' v''
+      proof -
+        have \<open>(\<exists>xa. (\<exists>u v. xa = u * v \<and> u \<in> {1} \<and> v \<in> \<I> I2 (r * x) \<and> u ## v) \<and> r ## x \<and> x \<in> D' \<and> (xa, y) \<in> S2)\<close>
+          by (simp, rule exI[where x=xb], simp add: prems2 prems)
+        note prems(2)[THEN spec[where x=x],THEN spec[where x=r],THEN spec[where x=\<open>{1}\<close>], THEN spec[where x=y],
+                THEN mp, OF this]
+        then show ?thesis
+          apply clarsimp
+          using prems2(3) prems2(4) prems2(5) by auto
+      qed .
+  qed .
+
+lemma sep_refinement_stepwise':
+  \<open> S1 \<r>\<e>\<f>\<i>\<n>\<e>\<s> S2 \<w>.\<r>.\<t> I1 \<i>\<n> D
+\<Longrightarrow> S2' \<r>\<e>\<f>\<i>\<n>\<e>\<s> S3 \<w>.\<r>.\<t> I2 \<i>\<n> D'
+\<Longrightarrow> refinement_projection I2 D' \<subseteq> D
+\<Longrightarrow> S2 \<subseteq> S2'
+\<Longrightarrow> S1 \<r>\<e>\<f>\<i>\<n>\<e>\<s> S3 \<w>.\<r>.\<t> (I1 o\<^sub>\<I> I2) \<i>\<n> D'\<close>
+  using refinement_sub_fun sep_refinement_stepwise
+  by metis
+
+
+
+subsubsection \<open>Function, pointwise\<close>
+
+definition "\<F>_fun' I = Interp (\<lambda>f. prod (\<lambda>x. \<I> (I x) (f x)) (dom1 f))"
+
+lemma \<F>_fun'_\<I>[simp]: "\<I> (\<F>_fun' I) = (\<lambda>f. prod (\<lambda>x. \<I> (I x) (f x)) (dom1 f))"
+  unfolding \<F>_fun'_def by (rule Interp_inverse) (simp add: Interpretation_def)
+
+lemma \<F>_fun'_split:
+  " finite (dom1 f)
+\<Longrightarrow> \<I> (\<F>_fun' I) f = \<I> (\<F>_fun' I) (f(k:=1)) * \<I> (I k) (f k)
+   \<and> \<I> (\<F>_fun' I) (f(k:=1)) ## \<I> (I k) (f k)"
+  for f :: "'a \<Rightarrow> 'b::sep_algebra"
+  by simp (smt (verit, best) Interp_one dom1_upd fun_upd_triv mult.comm_neutral mult.commute prod.insert_remove)
+
+
+definition "\<F>_fun I = \<F>_fun' (\<lambda>_. I)"
+
+lemma \<F>_fun_\<I>[simp]: "\<I> (\<F>_fun I) = (\<lambda>f. prod (\<I> I o f) (dom1 f))"
+  unfolding \<F>_fun_def by simp
+
+lemma \<F>_fun_split:
+  " finite (dom1 f)
+\<Longrightarrow> \<I> (\<F>_fun I) f = \<I> (\<F>_fun I) (f(k:=1)) * \<I> I (f k)
+  \<and> \<I> (\<F>_fun I) (f(k:=1)) ## \<I> I (f k)"
+  for f :: "'a \<Rightarrow> 'b::sep_algebra"
+  unfolding \<F>_fun_def using \<F>_fun'_split .
+
+lemma \<F>_interp_fun_\<I>_1_fupdt[simp]: "\<I> (\<F>_fun I) (1(k:=v)) = \<I> I v" by simp
+
+
+definition "\<F>_pointwise I = Interp (\<lambda>f. {g. \<forall>x. g x \<in> \<I> I (f x) })"
+
+lemma \<F>_pointwise_\<I>[simp]:
+  "\<I> (\<F>_pointwise I) = (\<lambda>f. {g. \<forall>x. g x \<in> \<I> I (f x) })"
+  unfolding \<F>_pointwise_def
+  by (rule Interp_inverse) (auto simp add: Interpretation_def one_fun_def fun_eq_iff)
+
+
+definition "\<F>_pointwise' I = Interp (\<lambda>f. {g. \<forall>x. g x \<in> \<I> (I x) (f x) })"
+
+lemma \<F>_pointwise'_\<I>[simp]:
+  "\<I> (\<F>_pointwise' I) = (\<lambda>f. {g. \<forall>x. g x \<in> \<I> (I x) (f x) })"
+  unfolding \<F>_pointwise'_def
+  by (rule Interp_inverse) (auto simp add: Interpretation_def one_fun_def fun_eq_iff)
+
+
+
+subsubsection \<open>Pairwise\<close>
+
+definition "\<F>_pair I1 I2 = Interp (\<lambda>(x,y). \<I> I1 x * \<I> I2 y) "
+
+lemma \<F>_pair_\<I>[simp]: "\<I> (\<F>_pair I1 I2) = (\<lambda>(x,y). \<I> I1 x * \<I> I2 y)"
+  for I1 :: "('a::one,'b::sep_monoid) interp"
+  unfolding \<F>_pair_def
+  by (rule Interp_inverse) (simp add: Interpretation_def one_prod_def)
+
+notation \<F>_pair (infixl "\<bullet>\<^sub>\<F>" 50)
+
+
+subsubsection \<open>Option\<close>
+
+definition "\<F>_option I = Interp (case_option 1 I)"
+
+lemma \<F>_option_\<I>[simp]: "\<I> (\<F>_option I) = (case_option 1 I)"
+  unfolding \<F>_option_def
+  by (rule Interp_inverse) (simp add: Interpretation_def)
+
+
+definition "\<F>_optionwise I = Interp (\<lambda>x. case x of Some x' \<Rightarrow> Some ` I x' | _ \<Rightarrow> {None})"
+
+lemma \<F>_optionwise_\<I>[simp]:
+  "\<I> (\<F>_optionwise I) = (\<lambda>x. case x of Some x' \<Rightarrow> Some ` I x' | _ \<Rightarrow> {None})"
+  unfolding \<F>_optionwise_def
+  by (rule Interp_inverse) (auto simp add: Interpretation_def)
+
+
+(* subsubsection \<open>Partiality\<close>
+
+definition "fine I = Interp (case_fine (\<I> I) {})"
+lemma fine_\<I>[simp]: "\<I> (fine I) = case_fine (\<I> I) {}"
+  unfolding fine_def by (rule Interp_inverse) (simp add: Interpretation_def one_fine_def)
+
+definition "defined I = Interp (\<lambda>x. Fine ` \<I> I x)"
+lemma defined_\<I>[simp]: "\<I> (defined I) = (\<lambda>x. Fine ` \<I> I x)"
+  unfolding defined_def
+  by (rule Interp_inverse) (auto simp add: Interpretation_def one_fine_def)
+
+definition "partialwise I = \<F>_fine (defined I)"
+lemma partialwise_\<I>[simp]: "\<I> (partialwise I) (Fine x) = { Fine y |y. y \<in> \<I> I x }"
+  unfolding partialwise_def by auto
+*)
+
+subsubsection \<open>Functional Fiction\<close>
+
+definition \<open>\<F>_functional \<psi> = Interp (\<lambda>x. {y. x = \<psi> y})\<close>
+
+lemma (in kernel_is_1) \<F>_functional_\<I>[simp]:
+  \<open>\<I> (\<F>_functional \<psi>) = (\<lambda>x. {y. x = \<psi> y})\<close>
+  unfolding \<F>_functional_def
+  by (rule Interp_inverse, simp add: Interpretation_def one_set_def set_eq_iff inj_at_1)
+
+lemma map_option_inj_at_1[simp]:
+  \<open>kernel_is_1 (map_option f)\<close>
+  unfolding one_option_def kernel_is_1_def
+  by (simp add: split_option_all)
+
+
+definition "\<F>_share s = (case s of Share w v \<Rightarrow> if w = 1 then {v} else {})"
+
+lemma \<F>_share_\<I>[simp]: "\<F>_share (Share w v) = (if w = 1 then {v} else {})"
+  unfolding \<F>_share_def by simp
+
+(* lemma In_ficion_fine [simp]:
+  \<open>x \<in> (case some_fine of Fine y \<Rightarrow> f y | Undef \<Rightarrow> {})
+        \<longleftrightarrow> (\<exists>y. some_fine = Fine y \<and> x \<in> f y)\<close>
+  by (cases some_fine; simp)
+*)
+
+subsubsection \<open>Agreement\<close>
+
+definition \<open>\<F>_agree = (\<lambda>x. case x of agree x' \<Rightarrow> {x'})\<close>
+
+
+
+
+
+end
