Phi_Algebras/Phi_Spec_Pre.thy
@@ -1,0 +1,13 @@
+theory Phi_Spec_Pre
+  imports Main
+begin
+
+definition Subjection :: " 'p set \<Rightarrow> bool \<Rightarrow> 'p set " (infixl "\<s>\<u>\<b>\<j>" 15)
+  where " (T \<s>\<u>\<b>\<j> P) = {p. p \<in> T \<and> P}"
+
+lemma Subjection_expn:
+  "p \<in> (T \<s>\<u>\<b>\<j> P) \<longleftrightarrow> p \<in> T \<and> P"
+  unfolding Subjection_def by simp
+
+
+end
